theories/Patterns.v
@@ -1,11 +1,11 @@
 From Vellvm Require Import Syntax ScopeTheory Semantics.
 From ITree Require Import ITree Eq.
-From Pattern Require Import IdModule MapCFG Head Focus.
+From Pattern Require Import IdModule MapCFG Head Focus Block.
 Require Import FSets.FMapAVL FSets.FMapFacts.
 Require Import List.
 Import ListNotations.
 Import Map MapF MapF.P MapF.P.F.
-Import IdOT MapCFG Head Focus.
+Import IdOT MapCFG Head Focus Block.
 
 (* Pattern definition *)
 
@@ -15,7 +15,8 @@ Inductive Pat : Type -> Type :=
   | Head: forall {S}, Pat S -> Pat (blk * S)
   | Focus: forall {S}, Pat S -> Pat (map_cfg * S)
   | Map: forall {S} {T}, Pat S -> (S -> T) -> Pat T
-  .
+  | Block: forall {S}, Pat S -> Pat (blk * S)
+.
 
 Notation "□" := Graph.
 Notation "P 'when' b" := (When P b) (at level 45).
@@ -52,41 +53,43 @@ Qed.
 Fixpoint MatchAll {S} (P: Pat S) (g: map_cfg) : list S :=
   match P with
     | □ => [g]
-    | Head _ p => flat_map_r (MatchAll p) (find_heads g)
+    | Head _ p => flat_map_r (MatchAll p) (heads g)
     | Focus _ p => flat_map_r (MatchAll p) (focus g)
     | p when f => List.filter f (MatchAll p g) 
     | Map _ _ p f => List.map f (MatchAll p g)
+    | Block _ p => flat_map_r (MatchAll p) (blocks g)
 end.
 
 (* Correction de MatchAll *)
 
-Theorem pat_graph_correct: forall G G', G' ∈ (MatchAll □ G) -> G' = G.
+Theorem Pat_Graph_correct: forall G G', G' ∈ (MatchAll □ G) -> G' = G.
 Proof.
   cbn. intros G G' H. destruct H; now destruct H.
 Qed.
 
-Theorem pat_head_correct {S}:
+Theorem Pat_Head_correct {S}:
   forall (G: map_cfg) (P: Pat S) (b:blk) s, wf_map_cfg G ->
   (b, s) ∈ (MatchAll (Head P) G) <->
   exists G', is_head G G' b /\ s ∈ (MatchAll P G').
 Proof.
-  intros G P b s Hwf. setoid_rewrite <-head_correct;trivial. apply in_flat_map_r.
+  intros G P b s Hwf. setoid_rewrite <- heads_correct;trivial. apply in_flat_map_r.
 Qed.
 
-Theorem pat_focus_correct {S}:
+Theorem Pat_Focus_correct {S}:
   forall (G G1: map_cfg) (P:Pat S) s, wf_map_cfg G ->
   (G1, s) ∈ (MatchAll (Focus P) G) <-> exists G2, is_focus G G1 G2 /\ s ∈ (MatchAll P G2).
 Proof.
   intros G G1 P s Hwf. setoid_rewrite <-focus_correct;trivial. apply in_flat_map_r.
 Qed.
 
-Theorem pat_when_correct {S}:
+Theorem Pat_When_correct {S}:
   forall (P: Pat S) f x G,
   x ∈ (MatchAll (When P f) G) <-> x ∈ (MatchAll P G) /\ f x = true.
 Proof.
   intros. apply filter_In.
 Qed.
-Theorem pat_map_correct {S T}:
+
+Theorem Pat_Map_correct {S T}:
   forall (P: Pat S) (f: S -> T) x G,
   x ∈ (MatchAll (Map P f) G) <-> exists y, f y = x /\ y ∈ (MatchAll P G).
 Proof.
@@ -95,7 +98,13 @@ Proof.
   - intros [y [H1 H2]]. subst x. now apply in_map.
 Qed.
 
-(* Block Fusion Pattern *)
+Theorem Pat_Block_correct {S}:
+  forall (G: map_cfg) (P: Pat S) (b:blk) s, wf_map_cfg G ->
+  (b, s) ∈ (MatchAll (Block P) G) <->
+  exists G', is_block G G' b /\ s ∈ (MatchAll P G').
+Proof.
+  intros. setoid_rewrite <-blocks_correct;trivial. apply in_flat_map_r.
+Qed.
 
 Definition map_cfg_to_ocfg: map_cfg -> ocfg. Admitted.
 
