theories/Block.v
@@ -1,0 +1,19 @@
+From Vellvm Require Import Syntax ScopeTheory Semantics.
+From ITree Require Import ITree Eq.
+Require Import FSets.FMapAVL FSets.FMapFacts.
+Require Import List.
+Import ListNotations.
+From Pattern Require Import IdModule MapCFG.
+Import Map MapF MapF.P MapF.P.F.
+Import IdOT MapCFG.
+
+
+Definition blocks_aux (G: map_cfg) : _ -> (blk*map_cfg) := fun '(id, b) => (b, remove id G).
+
+Definition blocks (G: map_cfg): list (blk*map_cfg) := List.map (blocks_aux G) (elements G).
+
+Definition is_block (G G': map_cfg) b := MapsTo b.(blk_id) b G /\ G' ≡ (remove b.(blk_id) G).
+
+Lemma blocks_correct: forall G G' b, wf_map_cfg G -> ((b, G') ∈ (blocks G) <-> is_block G G' b).
+Proof.
+Admitted.
