theories/CCstP.v
@@ -1,0 +1,28 @@
+From Vellvm Require Import Syntax ScopeTheory Semantics.
+From ITree Require Import ITree Eq.
+From Pattern Require Import IdModule MapCFG Head Focus Patterns.
+Require Import FSets.FMapAVL FSets.FMapFacts.
+Require Import List.
+Import ListNotations.
+Import Map MapF MapF.P MapF.P.F.
+Import IdOT MapCFG Head Focus Patterns.
+
+(* Print texp.
+Print exp.
+Search exp. *)
+
+Notation exp := (texp dtyp).
+
+Definition IsTrue: exp -> Prop. Admitted.
+
+Definition eqb_exp : exp -> exp -> bool. Admitted.
+
+Lemma eqb_exp_eq : forall e e', eqb_exp e e' = true -> IsTrue e -> IsTrue e'. Admitted.
+
+Definition is_branch_using e (b: blk) := match b.(blk_term) with
+    | TERM_Br e' _ _ => eqb_exp e e'
+    | _ => false
+end.
+
+Definition CCstP {S} (P:Pat S) e := (Block P) when (fun '(B, _) => is_branch_using e B).
+
